<?xml version="1.0" encoding="UTF-8" ?>

<!--********************************************************************
© 2024 Jeremy Sylvestre

Permission is granted to copy, distribute and/or modify this document
under the terms of the GNU Free Documentation License, Version 1.3 or
any later version published by the Free Software Foundation; with no
Invariant Sections, no Front-Cover Texts, and no Back-Cover Texts. A
copy of the license is included in the appendix entitled “GNU Free
Documentation License” that appears in the output document of this
PreTeXt source code. All trademarks™ are the registered® marks of their
respective owners.
*********************************************************************-->

<exercisegroup cols="2">
<title>Isolating via matrix algebra</title>

<introduction><p>
	In each case,
	use matrix algebra to isolate and determine the unknown variable matrix.
</p></introduction>

<exercise>

	<statement><p><m>\displaystyle
		\begin{amatrix}{rr}
			-8 \amp  7 \\
			 0 \amp -3
		\end{amatrix}
		- 2 X
		=
		\begin{amatrix}{rr}
			 5 \amp 0 \\
			-6 \amp 8
		\end{amatrix}
	</m></p></statement>

	<solution><p>
		It's less messy to perform algebraic manipulations with letters,
		so assign
		<md><mrow>
			A \amp =
			\begin{amatrix}{rr}
				-8 \amp  7 \\
				 0 \amp -3
			\end{amatrix}
			\text{,}
			\amp
			B \amp =
			\begin{amatrix}{rr}
				5 \amp 0 \\
				-6 \amp 8
			\end{amatrix}
			\text{.}
		</mrow></md>
		Then we have
		<md alignment="gather">
			<mrow> A - 2 X = B </mrow>
			<mrow> A - B = 2 X </mrow>
			<mrow> X = \tfrac{1}{2} (A - B) </mrow>
		</md>
		and we may calculate
		<md>
			<mrow>
				A - B \amp =
				\begin{amatrix}{rr}
					-8 \amp  7 \\
					 0 \amp -3
				\end{amatrix}
				-
				\begin{amatrix}{rr}
					 5 \amp 0 \\
					-6 \amp 8
				\end{amatrix}
			</mrow>

			<mrow>
				\amp =
				\begin{amatrix}{rr}
					-13 \amp   7 \\
					  6 \amp -11
				\end{amatrix}
			</mrow>

		</md>,
		<md>

			<mrow> X \amp = \tfrac{1}{2} (A - B) </mrow>

			<mrow>
				\amp =
				\frac{1}{2}
				\begin{amatrix}{rr}
					-13 \amp   7 \\
					  6 \amp -11
				\end{amatrix}
			</mrow>

			<mrow>
				\amp =
				\begin{bmatrix}
					-13/2 \amp   7/2 \\
					   3  \amp -11/2
				\end{bmatrix}
			</mrow>

		</md>.
	</p></solution>

</exercise>

<exercise>

	<statement><p><m>\displaystyle
		5 \utrans{X}
		+
		\begin{amatrix}{rr}
			-3 \amp -7 \\
			 3 \amp  6 \\
			-1 \amp -1
		\end{amatrix}
		=
		\zerovec
	</m></p></statement>

	<solution><p>
		It's less messy to perform algebraic manipulations with letters,
		so assign
		<me>
			A =
			\begin{amatrix}{rr}
				-3 \amp -7 \\
				 3 \amp  6 \\
				-1 \amp -1
			\end{amatrix}
		</me>.
		Then we have
		<md alignment="gather">
			<mrow> 5 \utrans{X} + A = \zerovec </mrow>
			<mrow> 5 \utrans{X} = - A </mrow>
			<mrow> \utrans{X} = - \tfrac{1}{5} A </mrow>
			<mrow> \utrans{(\utrans{X})} = \utrans{(- \tfrac{1}{5} A)} </mrow>
			<mrow> X = - \tfrac{1}{5} \utrans{A} </mrow>
		</md>
		and we may calculate
		<md>

			<mrow>
				\utrans{A} \amp =
				\utrans{\begin{amatrix}{rr}
					-3 \amp -7 \\
					 3 \amp  6 \\
					-1 \amp -1
				\end{amatrix}}
			</mrow>

			<mrow>
				\amp =
				\begin{amatrix}{rrr}
					-3 \amp 3 \amp -1 \\
					-7 \amp 6 \amp -1
				\end{amatrix}
			</mrow>

		</md>,

		<md>

			<mrow> X \amp = - \tfrac{1}{5} \utrans{A} </mrow>

			<mrow>
				\amp =
				- \frac{1}{5}
				\begin{amatrix}{rrr}
					-3 \amp 3 \amp -1 \\
					-7 \amp 6 \amp -1
				\end{amatrix}
			</mrow>

			<mrow>
				\amp =
				\begin{amatrix}{rrr}
					3/5 \amp -3/5 \amp -1/5 \\
					7/5 \amp -6/5 \amp -1/5
				\end{amatrix}
			</mrow>

		</md>.
	</p></solution>

</exercise>

</exercisegroup>
