<?xml version="1.0" encoding="UTF-8" ?>

<!--********************************************************************
© 2016–2024 Jeremy Sylvestre

Permission is granted to copy, distribute and/or modify this document
under the terms of the GNU Free Documentation License, Version 1.3 or
any later version published by the Free Software Foundation; with no
Invariant Sections, no Front-Cover Texts, and no Back-Cover Texts. A
copy of the license is included in the appendix entitled “GNU Free
Documentation License” that appears in the output document of this
PreTeXt source code. All trademarks™ are the registered® marks of their
respective owners.
*********************************************************************-->


<section xml:id="section-inverses-examples">

<assemblage><title>In this section</title><p><ul>
<li><xref ref="subsection-inverses-examples-2x2" /><nbsp /><nbsp />
<em><xref text="title" ref="subsection-inverses-examples-2x2" /></em></li>
<li><xref ref="subsection-inverses-examples-solving-sys" /><nbsp /><nbsp />
<em><xref text="title" ref="subsection-inverses-examples-solving-sys" /></em></li>
<li><xref ref="subsection-inverses-examples-solving-alg-eqns" /><nbsp /><nbsp />
<em><xref text="title" ref="subsection-inverses-examples-solving-alg-eqns" /></em></li>
</ul></p></assemblage>


<title>Examples</title>

<subsection xml:id="subsection-inverses-examples-2x2">
<title>Inverses of <m>2\times 2</m> matrices</title>

<p>
There is a general formula for the inverse of a <m>2\times 2</m> formula:
<md><mrow>
	A \amp = \begin{bmatrix} a \amp b \\ c \amp d \end{bmatrix}
	\amp\amp\implies\amp
	\inv{A} \amp = \frac{1}{ad-bc} \, \left[\begin{array}{rr} d \amp -b \\ -c \amp a \end{array}\right].
</mrow></md>
The formula <m>ad-bc</m> in the denominator of the scalar multiple in this inverse formula is called the
<term>determinant</term><idx><h>determinant</h></idx> of <m>A</m>.
Clearly the formula does not work when the determinant of <m>A</m> is <m>0</m>,
since we cannot divide by zero.
In fact, in
<xref ref="chapter-elem-matrices" />
it will be possible for us to prove that <m>A</m> is <em>not</em> invertible when <m>ad-bc=0</m>.
There are similar formulas for inverses of larger matrices,
but they are too complicated to write down explicitly.
We will study the general theory of determinants and related inversion formulas in
<xref first="chapter-det" last="chapter-more-det">Chapters</xref>.
</p>

<example><title>Using the <m>2 \times 2</m> inversion formula</title><statement><p>
	Matrix <m>A</m> below is invertible,
	and its inverse is given.
	Watch for double negatives when computing <m>ad-bc</m>!
	<md>
		<mrow>
			A \amp = \left[\begin{array}{rr} -5 \amp 1 \\ -3 \amp 2 \end{array}\right]
			\amp\amp\implies\amp
			\inv{A} \amp = \frac{1}{(-5)(2) - (1)(-3)}\,
			\left[\begin{array}{rr} 2 \amp -1 \\ 3 \amp -5 \end{array}\right]
		</mrow><mrow>
			\amp\amp\amp\amp
			\amp = -\frac{1}{7} \, \left[\begin{array}{rr} 2 \amp -1 \\ 3 \amp -5 \end{array}\right]
		</mrow><mrow>
			\amp\amp\amp\amp
			\amp = \left[\begin{array}{rr} -2/7 \amp 1/7 \\ -3/7 \amp 5/7 \end{array}\right].
		</mrow>
	</md>
	Let's check that we have the correct inverse.
	To keep the computations simple,
	we'll leave the <m>-1/7</m> as a scalar multiple when expressing <m>\inv{A}</m>.
	<md>
		<mrow>
			\inv{A}A
			\amp =
			\left( -\frac{1}{7} \, \left[\begin{array}{rr} 2 \amp -1 \\ 3 \amp -5 \end{array}\right] \right)
			\left[\begin{array}{rr} -5 \amp 1 \\ -3 \amp 2 \end{array}\right]
			\amp
			A\inv{A}
			\amp =
			\left[\begin{array}{rr} -5 \amp 1 \\ -3 \amp 2 \end{array}\right]
			\left( -\frac{1}{7} \, \left[\begin{array}{rr} 2 \amp -1 \\ 3 \amp -5 \end{array}\right] \right)
		</mrow><mrow>
			\amp=
			-\frac{1}{7} \, \left[\begin{array}{rr} 2 \amp -1 \\ 3 \amp -5 \end{array}\right]
			\left[\begin{array}{rr} -5 \amp 1 \\ -3 \amp 2 \end{array}\right]
			\amp
			\amp=
			-\frac{1}{7}\,
			\left[\begin{array}{rr} -5 \amp 1 \\ -3 \amp 2 \end{array}\right]
			\left[\begin{array}{rr} 2 \amp -1 \\ 3 \amp -5 \end{array}\right]
		</mrow><mrow>
			\amp=
			-\frac{1}{7} \, \begin{bmatrix} -10+3 \amp 2-2 \\ -15+15 \amp 3-10 \end{bmatrix}
			\amp
			\amp=
			-\frac{1}{7} \, \begin{bmatrix} -10+3 \amp 5-5 \\ -6+6 \amp 3-10 \end{bmatrix}
		</mrow><mrow>
			\amp=
			-\frac{1}{7} \, \left[\begin{array}{rr} -7 \amp 0 \\ 0 \amp -7 \end{array}\right]
			\amp
			\amp=
			-\frac{1}{7} \, \left[\begin{array}{rr} -7 \amp 0 \\ 0 \amp -7 \end{array}\right]
		</mrow><mrow>
			\amp= \begin{bmatrix} 1 \amp 0 \\ 0 \amp 1 \end{bmatrix}
			\amp
			\amp= \begin{bmatrix} 1 \amp 0 \\ 0 \amp 1 \end{bmatrix}
		</mrow>
	</md>
	So, we have both <m>\inv{A}A=I</m> and <m>A\inv{A}=I</m>, as required.
</p></statement></example>

<example><title>Sometimes the <m>2 \times 2</m> inversion formula does not apply</title><statement><p>
	Consider matrix
	<me> B = \begin{bmatrix} 3 \amp 6 \\ 1 \amp 2 \end{bmatrix}. </me>
	For this matrix, we have
	<me> ad-bc = 3\cdot 2 - 6 \cdot 1 = 6-6 = 0. </me>
	So even though none of the entries of <m>B</m> are <m>0</m>,
	it is not invertible.
</p></statement></example>

</subsection>

<subsection xml:id="subsection-inverses-examples-solving-sys">
<title>Solving systems using inverses</title>

<p>
Just as we can solve the numerical equation <m>ax=b</m> as <m>x = \inv{a}b</m>,
we can solve a system of equations that is represented as a matrix equation <m>A\uvec{x} = \uvec{b}</m> using <m>\inv{A}</m>.
</p>

<example xml:id="example-inverses-solving-sys"><statement><p>
	Consider the system
	<me>
		\left\{\begin{array}{rcrcrcr}
			-5x \amp + \amp y \amp = \amp 3, \\
			-3x \amp + \amp 2y \amp = \amp -2.
		\end{array}\right.
	</me>
	The coefficient matrix for this system is
	<me> A = \left[\begin{array}{rr} -5 \amp 1 \\ -3 \amp 2 \end{array}\right], </me>
	which is conveniently the matrix for which we have already computed the inverse using the <m>2\times 2</m> inversion formula in
	<xref ref="subsection-inverses-examples-2x2" />.
	So we can solve the system as
	<md>
		<mrow>
			A\uvec{x}\amp=\uvec{b} \amp
			\amp\implies \amp
			\uvec{x} \amp= \inv{A}\uvec{b}
		</mrow><mrow>
			\amp\amp\amp\amp
			\amp = \left( -\frac{1}{7} \, \left[\begin{array}{rr} 2 \amp -1 \\ 3 \amp -5 \end{array}\right] \right)
			\left[\begin{array}{r} 3 \\ -2 \end{array}\right]
		</mrow><mrow>
			\amp\amp\amp\amp
			\amp = -\frac{1}{7} \, \left[\begin{array}{rr} 2 \amp -1 \\ 3 \amp -5 \end{array}\right]
			\left[\begin{array}{r} 3 \\ -2 \end{array}\right]
		</mrow><mrow>
			\amp\amp\amp\amp
			\amp = -\frac{1}{7} \, \begin{bmatrix} 8 \\ 19 \end{bmatrix}
		</mrow><mrow>
			\amp\amp\amp\amp
			\amp = \left[\begin{array}{r} -8/7 \\ -19/7 \end{array}\right],
		</mrow>
	</md>
	so that the system has one unique solution <m>x=-8/7</m>, <m>y=-19/7</m>.
</p></statement></example>

</subsection>

<subsection xml:id="subsection-inverses-examples-solving-alg-eqns">
<title>Solving other matrix equations using inverses</title>

<p> We can similarly use matrix algebra and inverses to solve matrix equations in general. </p>

<example xml:id="example-inverses-solving-alg-eqns"><statement><p>
	Consider the matrix equation
	<me>
		3 \left[\begin{array}{rr} 1 \amp 1 \\ -1 \amp 2 \end{array}\right]
		+ X \left[\begin{array}{rr} 0 \amp -3 \\ 2 \amp 1 \end{array}\right] = I.
	</me>
	Suppose we would like to solve this equation for the unknown <m>2\times 2</m> matrix <m>X</m>,
	where <m>I</m> is the <m>2 \times 2</m> identity matrix.
	</p><p>
	One approach to this problem would be to express <m>X</m> in terms of unknown entries,
	<me> X = \begin{bmatrix} a \amp b \\ c \amp d \end{bmatrix}, </me>
	and then set up four equations in the four unknowns <m>a,b,c,d</m>.
	This would lead to a system of equations that we could row reduce and solve.
	But it's easier just to use ordinary (matrix) algebra.
	Set
	<md><mrow>
		W  \amp = \left[\begin{array}{rr} 1 \amp 1\\-1 \amp 2 \end{array}\right], \amp
		Z  \amp = \left[\begin{array}{rr} 0 \amp -3\\2 \amp 1 \end{array}\right],
	</mrow></md>
	substitute these definitions into the given equation,
	and isolate <m>X</m> algebraically:
	<md>
		<mrow> 3W + XZ  \amp = I </mrow>
		<mrow> XZ  \amp = I - 3W </mrow>
		<mrow> XZ\inv{Z}  \amp = (I - 3W)\inv{Z} </mrow>
		<mrow> X  \amp = (I - 3W)\inv{Z}. </mrow>
	</md>
	Of course,
	this method wouldn't work if <m>Z</m> was not invertible,
	but it is,
	and we can calculate
	<md>
		<mrow>
			I - 3W  \amp = \begin{bmatrix} 1 \amp 0 \\ 0 \amp 1 \end{bmatrix}
			- 3\left[\begin{array}{rr} 1 \amp 1 \\ -1 \amp 2 \end{array}\right]
			\amp
			\inv{Z} \amp = \frac{1}{0\cdot 1 - (-3)\cdot 2}
			\left[\begin{array}{rr} 1 \amp 3 \\ -2 \amp 0 \end{array}\right]
		</mrow><mrow>
			\amp = \begin{bmatrix} 1 \amp 0 \\ 0 \amp 1 \end{bmatrix}
			- \left[\begin{array}{rr} 3 \amp 3 \\ -3 \amp 6 \end{array}\right]
			\amp
			\amp = \frac{1}{6} \left[\begin{array}{rr} 1 \amp 3\\-2 \amp 0 \end{array}\right].
		</mrow><mrow>
	 		\amp = \left[\begin{array}{rr} -2 \amp -3 \\ 3 \amp -5 \end{array}\right],
		</mrow>
	</md>
	From this we obtain
	<me>
		X
		= (I - 3W)\inv{Z}
		= \left[\begin{array}{rr} -2  \amp  -3 \\ 3  \amp  -5 \end{array}\right]
		\left( \frac{1}{6} \left[\begin{array}{rr} 1 \amp 3\\-2 \amp 0 \end{array}\right] \right)
		= \frac{1}{6} \left[\begin{array}{rr} 4 \amp -6\\ 13 \amp 9 \end{array}\right]
		= \left[\begin{array}{rr} 2/3 \amp -1 \\ 13/6 \amp 3/2 \end{array}\right].
	</me>
</p></statement></example>

</subsection>

</section>
