<?xml version="1.0" encoding="UTF-8" ?>

<!--********************************************************************
© 2016–2024 Jeremy Sylvestre

Permission is granted to copy, distribute and/or modify this document
under the terms of the GNU Free Documentation License, Version 1.3 or
any later version published by the Free Software Foundation; with no
Invariant Sections, no Front-Cover Texts, and no Back-Cover Texts. A
copy of the license is included in the appendix entitled “GNU Free
Documentation License” that appears in the output document of this
PreTeXt source code. All trademarks™ are the registered® marks of their
respective owners.
*********************************************************************-->


<section xml:id="section-vector-geom-theory"  xmlns:xi="http://www.w3.org/2001/XInclude">

<title>Theory</title>

<assemblage><title>In this section</title><p><ul>
<li><xref ref="subsection-vector-geom-theory-norm-and-dot-prod" /><nbsp /><nbsp />
<em><xref text="title" ref="subsection-vector-geom-theory-norm-and-dot-prod" /></em></li>
<li><xref ref="subsection-vector-geom-theory-inequalities" /><nbsp /><nbsp />
<em><xref text="title" ref="subsection-vector-geom-theory-inequalities" /></em></li>
</ul></p></assemblage>

<subsection xml:id="subsection-vector-geom-theory-norm-and-dot-prod">
<title>Norm and dot product</title>

<p> We'll begin with algebraic properties of norm and dot product. </p>

<proposition xml:id="proposition-vector-geom-norm-algebra">

	<title> Properties of the norm </title>

	<statement><p>
		The following are true for all vectors <m>\uvec{u}</m> and <m>\uvec{v}</m> in <m>\R^n</m> and all scalars <m>k</m>.
		<ol>
			<li xml:id="proposition-vector-geom-norm-algebra-nonneg">
				<m>\unorm{v} \ge 0</m>, and <m>\unorm{v} = 0</m> only for <m>\uvec{v} = 0</m>.
			</li>
			<li> <m>\norm{-\uvec{v}} = \unorm{v}</m>. </li>
			<li xml:id="proposition-vector-geom-norm-algebra-scalar-mul">
				<m>\norm{k\uvec{v}} = \abs{k}\unorm{v}</m>.
			</li>
			<li> <m>\norm{\uvec{v}-\uvec{u}} = \norm{\uvec{u}-\uvec{v}}</m>. </li>
		</ol>
	</p></statement>

	<!-- TODO proofs? or at least comment on proofs relative to Activities/Concepts/Examples ? -->

</proposition>

<warning><p>
	The norm is <em>not</em> additive;
	that is, it is <alert>not</alert> true in general that <m>\norm{\uvec{u}+\uvec{v}}</m> is equal to <m>\unorm{u}+\unorm{v}</m>.
	<em>Sometimes</em> the two quantities are equal, as you are asked to consider below,
	but the best we can say about the norm of a sum is contained in <xref ref="theorem-vector-geom-triangle-ineq" /> below.
</p></warning>

<proposition xml:id="proposition-vector-geom-dot-prod-algebra">

	<title> Algebra rules of the dot product </title>

	<statement><p>
		The following are true for all vectors <m>\uvec{u}</m>, <m>\uvec{v}</m>, and <m>\uvec{w}</m> in <m>\R^n</m>, and all scalars <m>k</m>.
		<ol cols="2">
			<li xml:id="proposition-vector-geom-dot-prod-algebra-commute">
				<m>\udotprod{v}{u} = \udotprod{u}{v}</m>.
			</li>
			<li xml:id="proposition-vector-geom-dot-prod-algebra-distrib-left-over-right">
				<m>\dotprod{\uvec{u}}{(\uvec{v}+\uvec{w})} = \udotprod{u}{v} + \udotprod{u}{w}</m>.
			</li>
			<li> <m>\dotprod{\uvec{u}}{(\uvec{v}-\uvec{w})} = \udotprod{u}{v} - \udotprod{u}{w}</m>. </li>
			<li xml:id="proposition-vector-geom-dot-prod-algebra-distrib-right-over-left">
				<m>\dotprod{(\uvec{u}+\uvec{v})}{\uvec{w}} = \udotprod{u}{w} + \udotprod{v}{w}</m>.
			</li>
			<li> <m>\dotprod{(\uvec{u}-\uvec{v})}{\uvec{w}} = \udotprod{u}{w} - \udotprod{v}{w}</m>. </li>
			<li xml:id="proposition-vector-geom-dot-prod-algebra-scalar-left">
				<m>\dotprod{(k\uvec{u})}{\uvec{v}} = k(\udotprod{u}{v})</m>.
			</li>
			<li xml:id="proposition-vector-geom-dot-prod-algebra-scalar-right">
				<m>\dotprod{\uvec{u}}{(k\uvec{v})} = k(\udotprod{u}{v})</m>.
			</li>
			<li xml:id="proposition-vector-geom-dot-prod-algebra-vs-norm">
				<m>\udotprod{v}{v} = \unorm{v}^2</m>.
			</li>
			<li> Both <m>\dotprod{\uvec{v}}{\zerovec} = 0</m> and <m>\dotprod{\zerovec}{\uvec{v}} = 0</m>. </li>
		</ol>
	</p></statement>

	<!-- TODO proofs? or at least comment on proofs relative to Activities/Concepts/Examples ? -->

</proposition>

</subsection>


<subsection xml:id="subsection-vector-geom-theory-inequalities">
<title>Vector geometry inequalities and uniqueness of vector angles</title>

<paragraphs><title>The Cauchy-Schwarz inequality</title>

<p>
Here we will state the Cauchy-Schwarz inequality in its usual form.
Note that this version applies to <em>every</em> pair of vectors,
even if one is (or both are) the zero vector.
</p>

<theorem xml:id="theorem-vector-geom-cauchy-schwarz">
	<idx><h>Cauchy-Schwarz inequality</h></idx>
	<idx><h>inequality</h><h>Cauchy-Schwarz</h></idx>
	<title>The Cauchy-Schwarz inequality</title>

	<statement><p>
		For every pair of vectors <m>\uvec{u}</m> and <m>\uvec{v}</m> in <m>\R^n</m>,
		we have <m>\abs{\udotprod{u}{v}} \le \unorm{u}\unorm{v}</m>.
	</p></statement>

	<proof>

		<p>
		We will show that <m>(\udotprod{u}{v})^2 \le (\unorm{u}\unorm{v})^2</m>.
		Once this is established, then for <m>\udotprod{u}{v}</m> to have a smaller square than <m>\unorm{u}\unorm{v}</m>,
		it must be smaller in magnitude.
		That is, <m>(\udotprod{u}{v})^2 \le (\unorm{u}\unorm{v})^2</m> can only be true if <m>\abs{\udotprod{u}{v}} \le \abs{\unorm{u}\unorm{v}}</m> is true.
		But since neither <m>\unorm{u}</m> nor <m>\unorm{v}</m> can be negative,
		we have <m>\abs{\unorm{u}\unorm{v}} = \unorm{u}\unorm{v}</m>,
		and so <me> \abs{\udotprod{u}{v}} \le \unorm{u}\unorm{v} </me> will be established.
		</p>

		<p>
		So, we will try to prove that <m>(\udotprod{u}{v})^2 \le (\unorm{u}\unorm{v})^2</m> is always true for every pair of vectors <m>\uvec{u}</m> and <m>\uvec{v}</m> in <m>\R^n</m>.
		We might as well assume that <m>\uvec{v}</m> is nonzero,
		since if it is zero then both <m>(\udotprod{u}{v})^2</m> and <m>(\unorm{u}\unorm{v})^2</m> are <m>0</m>,
		and the required inequality is true.
		In the case that <m>\uvec{v}</m> is nonzero, then also <m>\unorm{v}\neq 0</m>
		(<xref ref="proposition-vector-geom-norm-algebra-nonneg">Statement</xref>
		of
		<xref ref="proposition-vector-geom-norm-algebra" />),
		and we can form the vector
		<md><mrow>
			\uvec{w} \amp= \uvec{u}-a\uvec{v}, \amp
			\text{where } a \amp= \frac{\udotprod{u}{v}}{\unorm{v}^2}
		</mrow></md>
		without worry that we've accidentally divided by zero.
		We will find that <m>\unorm{w}^2</m> is related to the inequality we are trying to prove, so compute
		<md>
			<mrow>
				\unorm{w}^2
				\amp= \udotprod{w}{w}
				\amp \amp\text{(i)}
			</mrow><mrow>
				\amp= \dotprod{(\uvec{u}-a\uvec{v})}{(\uvec{u}-a\uvec{v})}
				\amp \amp\text{(ii)}
			</mrow><mrow>
				\amp= \dotprod{(\uvec{u}-a\uvec{v})}{\uvec{u}}
				- \dotprod{(\uvec{u}-a\uvec{v})}{(a\uvec{v})}
				\amp \amp\text{(iii)}
			</mrow><mrow>
				\amp= \udotprod{u}{u} - \dotprod{(a\uvec{v})}{\uvec{u}}
				- \bbrac{\dotprod{\uvec{u}}{(a\uvec{v})} - \dotprod{(a\uvec{v})}{(a\uvec{v})}}
				\amp \amp\text{(iv)}
			</mrow><mrow>
				\amp= \udotprod{u}{u} - a(\udotprod{v}{u}) - a(\udotprod{u}{v}) + a\bbrac{a(\udotprod{v}{v})}
				\amp \amp\text{(v)}
			</mrow><mrow>
				\amp= \udotprod{u}{u} - a(\udotprod{u}{v}) - a(\udotprod{u}{v}) + a^2(\udotprod{v}{v})
				\amp \amp\text{(vi)}
			</mrow><mrow>
				\amp= \unorm{u}^2 - 2a(\udotprod{u}{v}) + a^2\unorm{v}^2
				\amp \amp\text{(vii)}
			</mrow><mrow>
				\amp= \unorm{u}^2
				- 2\left(\frac{\udotprod{u}{v}}{\unorm{v}^2}\right)(\udotprod{u}{v})
				+ \left(\frac{\udotprod{u}{v}}{\unorm{v}^2}\right)^2\unorm{v}^2
				\amp \amp\text{(viii)}
			</mrow><mrow>
				\amp= \unorm{u}^2
				- 2\frac{(\udotprod{u}{v})^2}{\unorm{v}^2}
				+ \frac{(\udotprod{u}{v})^2}{\unorm{v}^2},
			</mrow><mrow>
				\amp= \unorm{u}^2 - \frac{(\udotprod{u}{v})^2}{\unorm{v}^2}
			</mrow>
		</md>,
		with justifications
		<ol marker="(i)">
			<li>
				<xref ref="proposition-vector-geom-dot-prod-algebra-vs-norm">Rule</xref>
				of
				<xref ref="proposition-vector-geom-dot-prod-algebra" />;
			</li>
			<li>using the definition of <m>\uvec{w}</m> above;</li>
			<li>
				<xref ref="proposition-vector-geom-dot-prod-algebra-distrib-left-over-right">Rule</xref>
				of
				<xref ref="proposition-vector-geom-dot-prod-algebra" />;
			</li>
			<li>
				<xref ref="proposition-vector-geom-dot-prod-algebra-distrib-right-over-left">Rule</xref>
				of
				<xref ref="proposition-vector-geom-dot-prod-algebra" />;
			</li>
			<li>
				<xref ref="proposition-vector-geom-dot-prod-algebra-scalar-left">Rule</xref>
				and
				<xref ref="proposition-vector-geom-dot-prod-algebra-scalar-right">Rule</xref>
				of
				<xref ref="proposition-vector-geom-dot-prod-algebra" />;
			</li>
			<li>
				<xref ref="proposition-vector-geom-dot-prod-algebra-commute">Rule</xref>
				of
				<xref ref="proposition-vector-geom-dot-prod-algebra" />;
			</li>
			<li>
				<xref ref="proposition-vector-geom-dot-prod-algebra-vs-norm">Rule</xref>
				of
				<xref ref="proposition-vector-geom-dot-prod-algebra" />;
				and
			</li>
			<li> using the definition of <m>a</m> above. </li>
		</ol>
		Now, <m>\unorm{w}^2</m> cannot be negative, so we have
		<md>
			<mrow>0 \amp\le \unorm{u}^2 - \frac{(\udotprod{u}{v})^2}{\unorm{v}^2}</mrow>
			<mrow>\frac{(\udotprod{u}{v})^2}{\unorm{v}^2} \amp\le \unorm{u}^2</mrow>
			<mrow>(\udotprod{u}{v})^2 \amp\le \unorm{u}^2\unorm{v}^2</mrow>
		</md>,
		where multiplying both sides of the second inequality by the non-negative quantity <m>\unorm{v}^2</m> does not change the direction of the inequality.
		</p>

		<p>
		Because <m>\udotprod{u}{v}</m> <em>could</em> be negative,
		we will change our last inequality above to
		<me>\abs{\udotprod{u}{v}}^2 \le (\unorm{u}\unorm{v})^2</me>.
		</p>

		<aside><title>Note</title><p>
			Squaring turns negative into positive anyway, so it doesn't matter if we introduce absolute value brackets to do that first.
		</p></aside>

		<p>
		In words, this inequality says that the square of one number is less than or equal to the square of another number.
		But when we square two numbers, the bigger number will always result in the bigger square (as long as neither number is negative).
		Since neither <m>\abs{\udotprod{u}{v}}</m> nor <m>\unorm{u}\unorm{v}</m> can be negative,
		the bigger number must be <m>\unorm{u}\unorm{v}</m> to result in a bigger square (or the two numbers could be equal).
		That is, <me>\abs{\udotprod{u}{v}} \le \unorm{u}\unorm{v}</me>.
		</p>

	</proof>

</theorem>

<corollary xml:id="corollary-vector-geom-unique-angle">
	<title> Uniqueness of angle measures </title>
	<statement><p>
		For every pair of nonzero vectors <m>\uvec{u}</m> and <m>\uvec{v}</m> in <m>\R^n</m>,
		there is one unique angle value <m>\theta</m> in the domain <m>0 \le \theta \le \pi</m> so that
		<me> \cos\theta = \frac{\udotprod{u}{v}}{\unorm{u}\unorm{v}} </me>.
	</p></statement>
</corollary>

</paragraphs>

<paragraphs><title>The triangle inequality</title>

<p>
Here is another commonly used inequality.
Remembering our view of sums of vectors as a chain of changes in position,
it basically says that the shortest path between two points in <m>\R^n</m> is the direct path.
</p>

<theorem xml:id="theorem-vector-geom-triangle-ineq">
	<idx><h>triangle inequality</h></idx>
	<idx><h>inequality</h><h>triangle</h></idx>
	<title>Triangle inequality</title>

	<statement>

		<p>
		For every pair of vectors <m>\uvec{u}</m> and <m>\uvec{v}</m> in <m>\R^n</m>,
		we have <m>\norm{\uvec{u}+\uvec{v}} \le \unorm{u} + \unorm{v}</m>.
		</p>

		<image label="image-vector-geom-theory-triangle" width="42.6%">
			<!-- description gets inserted as alt text in html img tag -->
			<description>Diagram of the triangle inequality.</description>
			<latex-image><xi:include href="theory.d/triangle.tex" parse="text" /></latex-image>
		</image>

		<aside><title>Check your understanding</title><p>
			Can you think of a situation where <m>\norm{\uvec{u}+\uvec{v}}</m> and <m>\unorm{u} + \unorm{v}</m> are exactly equal?
			Is this the only way this would happen?
		</p></aside>

	</statement>

	<proof>

		<p>
		As mentioned in this chapter, working with square roots algebraically is inconvenient,
		so we will work with the square of the norm <m>\norm{\uvec{u}+\uvec{v}}</m>,
		and use <xref ref="proposition-vector-geom-dot-prod-algebra" /> to avoid working directly with the components of our vectors.
		</p>

		<p>
		We have
		<md>
			<mrow>
				\norm{\uvec{u}+\uvec{v}}^2
				\amp= \dotprod{(\uvec{u}+\uvec{v})}{(\uvec{u}+\uvec{v})}
				\amp \amp\text{(i)}
			</mrow><mrow>
				\amp= \dotprod{(\uvec{u}+\uvec{v})}{\uvec{u}} + \dotprod{(\uvec{u}+\uvec{v})}{\uvec{v}}
				\amp \amp\text{(ii)}
			</mrow><mrow>
				\amp= \udotprod{u}{u} + \udotprod{v}{u} + \udotprod{u}{v} + \udotprod{v}{v}
				\amp \amp\text{(iii)}
			</mrow><mrow>
				\amp= \udotprod{u}{u} + 2\udotprod{u}{v} + \udotprod{v}{v}
				\amp \amp\text{(iv)}
			</mrow><mrow>
				\amp= \unorm{u}^2 + 2\udotprod{u}{v} + \unorm{v}^2
				\amp \amp\text{(v)}
			</mrow>
		</md>,
		with justifications
		<ol marker="(i)">
			<li>
				<xref ref="proposition-vector-geom-dot-prod-algebra-vs-norm">Rule</xref>
				of
				<xref ref="proposition-vector-geom-dot-prod-algebra" />;
			</li>
			<li>
				<xref ref="proposition-vector-geom-dot-prod-algebra-distrib-left-over-right">Rule</xref>
				of
				<xref ref="proposition-vector-geom-dot-prod-algebra" />;
			</li>
			<li>
				<xref ref="proposition-vector-geom-dot-prod-algebra-distrib-right-over-left">Rule</xref>
				of
				<xref ref="proposition-vector-geom-dot-prod-algebra" />;
			</li>
			<li>
				<xref ref="proposition-vector-geom-dot-prod-algebra-commute">Rule</xref>
				of
				<xref ref="proposition-vector-geom-dot-prod-algebra" />;
				and
			</li>
			<li>
				<xref ref="proposition-vector-geom-dot-prod-algebra-vs-norm">Rule</xref>
				of
				<xref ref="proposition-vector-geom-dot-prod-algebra" />.
			</li>
		</ol>
		</p>

		<p>
		Now, keep in mind that <m>\udotprod{u}{v}</m> is a number, and it may be positive, negative, or zero.
		But every number <m>x</m> satisfies
		<md><mrow tag="star" xml:id="equation-vector-geom-theory-abs-x-ineq"> x \le \abs{x} </mrow></md>,
		since if <m>x</m> is positive or zero then the two sides are equal,
		and if <m>x</m> is negative then obviously the negative number <m>x</m> must be less than the positive number <m>\abs{x}</m>.
		Applying this for <m>x = \udotprod{u}{v}</m>, we have <m>\udotprod{u}{v} \le \abs{\udotprod{u}{v}}</m>, and so
		<md>
			<mrow>
				\norm{\uvec{u}+\uvec{v}}^2
				\amp= \unorm{u}^2 + 2\udotprod{u}{v} + \unorm{v}^2
				\amp \amp\text{(i)}
			</mrow><mrow>
				\amp\le \unorm{u}^2 + 2\abs{\udotprod{u}{v}} + \unorm{v}^2
				\amp \amp\text{(ii)}
			</mrow><mrow>
				\amp\le \unorm{u}^2 + 2\unorm{u}\unorm{v} + \unorm{v}^2
				\amp \amp\text{(iii)}
			</mrow><mrow>
				\amp= (\unorm{u} + \unorm{v})^2
				\amp \amp\text{(iv)}
			</mrow>
		</md>,
		with justifications
		<ol marker="(i)">
			<li> continued from above; </li>
			<li> rule <xref ref="equation-vector-geom-theory-abs-x-ineq" />; </li>
			<li> <xref ref="theorem-vector-geom-cauchy-schwarz" text="title" />; and </li>
			<li> FOIL in reverse. </li>
		</ol>
		Following the chain of equalities and inequalities from beginning to end, we now have
		<me> \norm{\uvec{u}+\uvec{v}}^2 \le (\unorm{u} + \unorm{v})^2 </me>.
		In words, this says that the square of one number is less than or equal to the square of another number.
		But when we square two numbers, the bigger number will always result in the bigger square
		(as long as neither number is negative).
		Since neither <m>\norm{\uvec{u}+\uvec{v}}</m> nor <m>\unorm{u} + \unorm{v}</m> can be negative,
		the bigger number must be <m>\unorm{u} + \unorm{v}</m> to result in a bigger square (or the two numbers could be equal).
		That is, <me> \norm{\uvec{u}+\uvec{v}} \le \unorm{u} + \unorm{v} </me>.
		</p>

	</proof>

</theorem>

</paragraphs>

</subsection>

</section>
