<?xml version="1.0" encoding="UTF-8" ?>

<!--********************************************************************
© 2016–2024 Jeremy Sylvestre

Permission is granted to copy, distribute and/or modify this document
under the terms of the GNU Free Documentation License, Version 1.3 or
any later version published by the Free Software Foundation; with no
Invariant Sections, no Front-Cover Texts, and no Back-Cover Texts. A
copy of the license is included in the appendix entitled “GNU Free
Documentation License” that appears in the output document of this
PreTeXt source code. All trademarks™ are the registered® marks of their
respective owners.
*********************************************************************-->


<section xml:id="section-lintrans-matrix-examples">

<title>Examples</title>

<assemblage><title>In this section</title><p><ul>
<li><xref ref="subsection-lintrans-matrix-examples-computing" /><nbsp /><nbsp />
<em><xref text="title" ref="subsection-lintrans-matrix-examples-computing" /></em></li>
<li><xref ref="subsection-lintrans-matrix-examples-using" /><nbsp /><nbsp />
<em><xref text="title" ref="subsection-lintrans-matrix-examples-using" /></em></li>
</ul></p></assemblage>

<subsection xml:id="subsection-lintrans-matrix-examples-computing">
<title>Computing the matrix of a linear transformation</title>

<p>
Here we will carry out the computations of <xref ref="activity-lintrans-matrix-examples" />.
In that discovery activity,
the instruction to use the isomorphisms from <xref ref="activity-lintrans-matrix-coord-maps-and-inverses" />
amounts to choosing standard bases for each space
(and choosing the provided basis for <m>V</m> in <xref ref="activity-lintrans-matrix-examples-trig-exp-diff">Discovery</xref>).
We will work each example in two different ways <mdash />
using <xref ref="procedure-lintrans-matrix-concepts-compute" />,
but also by just considering input-output formulas.
</p>

<example xml:id="example-lintrans-matrix-computing">
	<title>From <xref ref="activity-lintrans-matrix-examples" /></title>
	<p><ol>
		<li>
			<p>
			In <xref ref="activity-lintrans-matrix-examples-M2-to-P2">Discovery</xref>,
			we considered <m>\funcdef{T}{\matrixring_2(\R)}{\poly_2(\R)}</m>
			defined by
			<me> T\left(\begin{bmatrix} a \amp b \\ c \amp d \end{bmatrix}\right) = (a + b) x^2 + (a + b + c) x - d </me>.
			Choosing the standard basis <m>\basisfont{S}</m> for domain space <m>\matrixring_2(\R)</m>
			and the choice <m>\basisfont{S}' = \{ x^2, x, 1 \}</m> of a standard basis for <m>\poly_2(\R)</m>,
			we create a chain of transformations
			<me> \R^4 \xrightarrow{\invcoordmap{S}} \matrixring_2(\R) \xrightarrow{T} \poly_2(\R) \xrightarrow{\coordmap{S'}} \R^3 </me>
			where a typical vector <m>(a,b,c,d)</m> in <m>\R^4</m> shuttles through the pipe by
			<me>
				\begin{bmatrix} a \\ b \\ c \\ d \end{bmatrix}
				\mapsto
				\begin{bmatrix} a \amp b \\ c \amp d \end{bmatrix}
				\mapsto
				(a + b) x^2 + (a + b + c) x - d
				\mapsto
				\begin{bmatrix} a + b \\ a + b + c \\ -d \end{bmatrix}
			</me>.
			So the composite transformation <m>\R^4 \to \R^3</m> has input-output formulas
			<me>
				\left\{\begin{array}{cclclclcl}
					y_1 \amp = \amp x_1 \amp + \amp x_2 \text{,} \\
					y_2 \amp = \amp x_1 \amp + \amp x_2 \amp + \amp x_3 \text{,} \\
					y_3 \amp = \amp \amp \amp \amp \amp \amp - \amp x_4 \text{.} \\
				\end{array}\right.
			</me>
			Using these formulas as rows,
			we obtain matrix
			<me>
				\matrixOf{T}{S'S}
				= \left[\begin{array}{rrrr}
					1 \amp 1 \amp 0 \amp  0 \\
					1 \amp 1 \amp 1 \amp  0 \\
					0 \amp 0 \amp 0 \amp -1
				\end{array}\right]
			</me>.
			</p><p>
			We should get the same result if we using <xref ref="procedure-lintrans-matrix-concepts-compute" />.
			First, compute the images of the four basis vectors in <m>\basisfont{S}</m>:
			<md>
				<mrow>
					T\left(\begin{bmatrix} 1 \amp 0 \\ 0 \amp 0 \end{bmatrix}\right)
					\amp = x^2 + x \text{,}
					\amp
					T\left(\begin{bmatrix} 0 \amp 1 \\ 0 \amp 0 \end{bmatrix}\right)
					\amp = x^2 + x \text{,}
				</mrow><mrow>
					T\left(\begin{bmatrix} 0 \amp 0 \\ 1 \amp 0 \end{bmatrix}\right)
					\amp = x \text{,}
					\amp
					T\left(\begin{bmatrix} 0 \amp 0 \\ 0 \amp 1 \end{bmatrix}\right)
					\amp = -1 \text{.}
				</mrow>
			</md>
			Relative to the chosen basis <m>\basisfont{S}'</m> of the codomain space <m>\poly_2(\R)</m>,
			we have coordinate vectors
			<md>
				<mrow>
					\matrixOf{T(E_{11})}{S'} \amp = \begin{bmatrix} 1 \\ 1 \\  0 \end{bmatrix} \text{,} \amp
					\matrixOf{T(E_{12})}{S'} \amp = \begin{bmatrix} 1 \\ 1 \\  0 \end{bmatrix} \text{,}
				</mrow><mrow></mrow><mrow>
					\matrixOf{T(E_{21})}{S'} \amp = \begin{bmatrix} 0 \\ 1 \\  0 \end{bmatrix} \text{,} \amp
					\matrixOf{T(E_{22})}{S'} \amp = \left[\begin{array}{r} 0 \\ 0 \\ -1 \end{array}\right]
				</mrow>
			</md>.
			Using these coordinate vectors as columns in a matrix,
			we obtain the same result for <m>\matrixOf{T}{S'S}</m> as before.
			</p>
		</li>
		<li>
			<p>
			In <xref ref="activity-lintrans-matrix-examples-P2-to-U2">Discovery</xref>,
			we considered
			<m>\funcdef{T}{\poly_2(\R)}{\uppermatring_2(\R)}</m>,
			for <m>\uppermatring_2(\R)</m> the space of <m>2 \times 2</m> upper triangular matrices,
			defined by
			<me> T(a x^2 + b x + c) = \begin{bmatrix} a - b \amp b + c \\ 0 \amp c - a \end{bmatrix} </me>.
			Again, we take <m>\basisfont{S} = \{ x^2, x, 1 \}</m> as a choice of standard basis for <m>\poly_2(\R)</m>,
			and choose <m>\basisfont{S}' = \{ E_{11}, E_{12}, E_{22} \}</m> as a basis for <m>\uppermatring_2(\R)</m>.
			With these choices,
			we create a chain of transformations
			<me> \R^3 \xrightarrow{\invcoordmap{S}} \poly_2(\R) \xrightarrow{T} \uppermatring_2(\R) \xrightarrow{\coordmap{S'}} \R^3 </me>
			where a typical vector <m>(a,b,c)</m> in <m>\R^3</m> shuttles through the pipe by
			<me>
				\begin{bmatrix} a \\ b \\ c \end{bmatrix}
				\mapsto
				a x^2 + b x + c
				\mapsto
				\begin{bmatrix} a - b \amp b + c \\ 0 \amp c - a \end{bmatrix}
				\mapsto
				\begin{bmatrix} a - b \\ b + c \\ c - a \end{bmatrix}
			</me>.
			So the composite transformation <m>\R^3 \to \R^3</m> has input-output formulas
			<me>
				\left\{\begin{array}{ccrcccl}
					y_1 \amp = \amp   x_1 \amp - \amp x_2 \text{,} \\
					y_2 \amp = \amp       \amp   \amp x_2 \amp + \amp x_3 \text{,} \\
					y_3 \amp = \amp - x_1 \amp \amp \amp + \amp x_3 \text{.} \\
				\end{array}\right.
			</me>
			Using these formulas as rows,
			we obtain matrix
			<me>
				\matrixOf{T}{S'S}
				= \left[\begin{array}{rrrr}
					 1 \amp -1 \amp 0 \\
					 0 \amp  1 \amp 1 \\
					-1 \amp  0 \amp 1
				\end{array}\right]
			</me>.
			</p><p>
			We should get the same result if we using <xref ref="procedure-lintrans-matrix-concepts-compute" />.
			First, compute the images of the three basis vectors in <m>\basisfont{S}</m>:
			<md><mrow>
				T(x^2) \amp = \left[\begin{array}{rr} 1 \amp 0 \\ 0 \amp -1 \end{array}\right] \text{,} \amp
				T(x) \amp = \left[\begin{array}{rr} -1 \amp 1 \\ 0 \amp 0 \end{array}\right] \text{,} \amp
				T(1) \amp = \begin{bmatrix} 0 \amp 1 \\ 0 \amp 1 \end{bmatrix} \text{.}
			</mrow></md>
			Relative to the chosen basis <m>\basisfont{S}'</m> of the codomain space <m>\uppermatring_2(\R)</m>,
			we have coordinate vectors
			<md><mrow>
				\matrixOf{T(x^2)}{S'} \amp = \left[\begin{array}{r} 1 \\ 0 \\ -1 \end{array}\right] \text{,} \amp
				\matrixOf{T(x)}{S'} \amp = \left[\begin{array}{r} -1 \\ 1 \\  0 \end{array}\right] \text{,} \amp
				\matrixOf{T(1)}{S'} \amp = \begin{bmatrix} 0 \\ 1 \\  1 \end{bmatrix}
			</mrow></md>.
			Using these coordinate vectors as columns in a matrix,
			we obtain the same result for <m>\matrixOf{T}{S'S}</m> as before.
			</p>
		</li>
		<li xml:id="example-lintrans-matrix-computing-diff">
			<p>
			In <xref ref="activity-lintrans-matrix-examples-trig-exp-diff">Discovery</xref>,
			we considered the differentiation operator <m>\funcdef{D}{V}{V}</m> on the space <m>V = \Span \{ e^x \sin x, e^x \cos x \}</m>.
			The provided spanning set for <m>V</m> is linearly independent (check!).
			Using this basis on both the <q>input</q> and <q>output</q> ends,
			we create a chain of transformations
			<me> \R^2 \xrightarrow{\invcoordmap{B}} V \xrightarrow{D} V \xrightarrow{\coordmap{B}} \R^2 </me>
			where a typical vector <m>(a,b)</m> in <m>\R^2</m> shuttles through the pipe by
			<me>
				\begin{bmatrix} a \\ b \end{bmatrix}
				\mapsto
				a e^x \sin x + b e^x \cos x
				\mapsto
				(a - b) e^x \sin x + (a + b) \cos x
				\mapsto
				\begin{bmatrix} a - b \\ a + b \end{bmatrix}
			</me>.
			So the composite transformation <m>\R^2 \to \R^2</m> has input-output formulas
			<me>
				\left\{\begin{array}{cclcl}
					y_1 \amp = \amp x_1 \amp - \amp x_2 \text{,} \\
					y_2 \amp = \amp x_1 \amp + \amp x_2 \text{.}
				\end{array}\right.
			</me>
			Using these formulas as rows,
			we obtain matrix
			<me>
				\matrixOf{T}{B}
				= \left[\begin{array}{rr}
					1 \amp -1 \\
					1 \amp  1
				\end{array}\right]
			</me>.
			</p><p>
			We should get the same result if we using <xref ref="procedure-lintrans-matrix-concepts-compute" />.
			First, compute the images of the two basis vectors in <m>\basisfont{S}</m>:
			<md>
				<mrow> D(e^x \sin x) \amp = e^x \sin x + e^x \cos x \text{,} </mrow>
				<mrow> D(e^x \cos x) \amp = - e^x \sin x + e^x \cos x \text{.} </mrow>
			</md>
			Relative to the basis <m>\basisfont{B}</m> of <m>V</m>,
			we have coordinate vectors
			<md><mrow>
				\matrixOf{D(e^x \sin x)}{B} \amp = \begin{bmatrix} 1 \\ 1 \end{bmatrix} \text{,} \amp
				\matrixOf{D(e^x \cos x)}{B} \amp = \left[\begin{array}{r} -1 \\ 1 \end{array}\right]
			</mrow></md>.
			Using these coordinate vectors as columns in a matrix,
			we obtain the same result for <m>\matrixOf{D}{B}</m> as before.
			</p>
		</li>
	</ol></p>
</example>

</subsection>

<subsection xml:id="subsection-lintrans-matrix-examples-using">
<title>Using the matrix of a linear transformation</title>

<p> We can use the matrix of a linear transformation to compute image vectors. </p>
<p>
In each of the following examples,
we consider the differentiation operator <m>\funcdef{D}{V}{V}</m> on the space <m>V = \Span \{ e^x \sin x, e^x \cos x \}</m>.
In <xref ref="example-lintrans-matrix-computing-diff" text="local">Part</xref>
of <xref ref="example-lintrans-matrix-computing" /> above,
we have already computed
<me>
	\matrixOf{D}{B}
	= \left[\begin{array}{rr}
		1 \amp -1 \\
		1 \amp  1
	\end{array}\right]
</me>,
where <m>\basisfont{B}</m> is the provided basis for <m>V</m>,
by simply computing the derivatives of the basis vectors.
This information should be enough to allow us to compute the derivative of every <em>linear combination</em> of the basis vectors by simple matrix multiplication,
and in fact will also allow us to compute <em>anti</em>derivatives,
since <m>\matrixOf{D}{B}</m> is invertible.
</p>

<example xml:id="example-lintrans-matrix-diff-once">
	<title>Computing an image vector</title>
	<p>
	Consider <m>f(x) = 3 e^x \sin x - e^x \cos x</m>,
	with
	<me> \matrixOf{f}{B} = \left[\begin{array}{r} 3 \\ -1 \end{array}\right] </me>.
	Then we can compute
	<me>
		\matrixOf{D(f)}{B}
		= \matrixOf{D}{B} \matrixOf{f}{B}
		= \left[\begin{array}{rr}
			1 \amp -1 \\
			1 \amp  1
		\end{array}\right]
		\left[\begin{array}{r} 3 \\ -1 \end{array}\right]
		= \begin{bmatrix} 4 \\ 2 \end{bmatrix}
	</me>.
	Converting this coordinate vector back into a linear combination,
	we find
	<me> D\bigl(f(x)\bigr) = 4 e^x \sin x + 2 e^x \cos x </me>.
	</p>
</example>

<example xml:id="example-lintrans-matrix-diff-twice">
	<title>Computing the image vector of a composition</title>
	<p>
	Again consider <m>f(x) = 3 e^x \sin x - e^x \cos x</m>.
	What if we would like to compute the <em>second</em> derivative of <m>f(x) = 3 e^x \sin x - e^x \cos x</m>?
	We could of course just multiply the resulting coordinate vector from <xref ref="example-lintrans-matrix-diff-once" />
	by <m>\matrixOf{D}{B}</m> again.
	But let's proceed as if we had not already calculated <m>D(f)</m>.
	</p><p>
	Since the second derivative of <m>f</m> is <me>D\bigl(D(f)\bigr) = D^2(f)</me>,
	we can compute
	<me>
		\matrixOf{D^2}{B}
		= (\matrixOf{D}{B})^2
		= \left[\begin{array}{rr}
			1 \amp -1 \\
			1 \amp  1
		\end{array}\right]^2
		= \left[\begin{array}{rr}
			0 \amp -2 \\
			2 \amp  0
		\end{array}\right]
	</me>.
	Then from this we can compute
	<me>
		\matrixOf{D^2(f)}{B}
		= \matrixOf{D^2}{B} \matrixOf{f}{B}
		= \left[\begin{array}{rr}
			0 \amp -2 \\
			2 \amp  0
		\end{array}\right]
		\left[\begin{array}{r} 3 \\ -1 \end{array}\right]
		= \begin{bmatrix} 2 \\ 6 \end{bmatrix}
	</me>.
	Converting this coordinate vector back into a linear combination,
	we find
	<me> D^2\bigl(f(x)\bigr) = 2 e^x \sin x + 6 e^x \cos x </me>.
	</p>
</example>

<example xml:id="example-lintrans-matrix-antidiff">
	<title>Computing the image vector of the inverse of an operator</title>
	<p>
	Once again consider <m>f(x) = 3 e^x \sin x - e^x \cos x</m>.
	Since <m>\matrixOf{D}{B}</m> is invertible,
	so must be operator <m>D</m>.
	And if <m>D</m> represents differentiation,
	then <m>\inv{D}</m> must represent antidifferentiation,
	so computing <m>\inv{D}(f)</m> will be the antiderivative of <m>f(x)</m>.
	</p><p>
	First compute
	<me>
		\matrixOf{\inv{D}}{B}
		= \invmatrixOf{D}{B}
		= \inv{\left[\begin{array}{rr} 1 \amp -1 \\ 1 \amp  1 \end{array}\right]}
		= \frac{1}{2} \, \left[\begin{array}{rr} 1 \amp 1 \\ -1 \amp  1 \end{array}\right]
	</me>.
	With this,
	we can compute
	<me>
		\matrixOf{\inv{D}(f)}{B}
		= \matrixOf{\inv{D}}{B} \matrixOf{f}{B}
		= \frac{1}{2} \, \left[\begin{array}{rr} 1 \amp 1 \\ -1 \amp  1 \end{array}\right]
		\left[\begin{array}{r} 3 \\ -1 \end{array}\right]
		= \left[\begin{array}{r} 1 \\ -2 \end{array}\right]
	</me>.
	Converting this coordinate vector back into a linear combination,
	we find that the antiderivative of <m>f</m> is
	<me> \inv{D}\bigl(f(x)\bigr) = e^x \sin x - 2 e^x \cos x </me>.
	</p>
</example>

</subsection>

</section>
