<?xml version="1.0" encoding="UTF-8" ?>

<!--********************************************************************
© 2016–2023 Jeremy Sylvestre

Permission is granted to copy, distribute and/or modify this document
under the terms of the GNU Free Documentation License, Version 1.3 or
any later version published by the Free Software Foundation; with no
Invariant Sections, no Front-Cover Texts, and no Back-Cover Texts. A
copy of the license is included in the appendix entitled “GNU Free
Documentation License” that appears in the output document of this
PreTeXt source code. All trademarks™ are the registered® marks of their
respective owners.
*********************************************************************-->

<section xml:id="section-complex-appendix-field">
<title>The field of complex numbers</title>

<assemblage><title>In this section</title><p><ul>
<li><xref ref="subsection-complex-appendix-field-def" /><nbsp /><nbsp />
<em><xref text="title" ref="subsection-complex-appendix-field-def" /></em></li>
<li><xref ref="subsection-complex-appendix-field-ops" /><nbsp /><nbsp />
<em><xref text="title" ref="subsection-complex-appendix-field-ops" /></em></li>
<li><xref ref="subsection-complex-appendix-field-div" /><nbsp /><nbsp />
<em><xref text="title" ref="subsection-complex-appendix-field-div" /></em></li>
<li><xref ref="subsection-complex-appendix-field-props" /><nbsp /><nbsp />
<em><xref text="title" ref="subsection-complex-appendix-field-props" /></em></li>
<li><xref ref="subsection-complex-appendix-field-poly" /><nbsp /><nbsp />
<em><xref text="title" ref="subsection-complex-appendix-field-poly" /></em></li>
</ul></p></assemblage>

<introduction><p>
	Now that we have a new number,
	let's let it out to play in the <term>field</term> with all the other numbers.
</p></introduction>

<subsection xml:id="subsection-complex-appendix-field-def">
<title> Definition of the field </title>

<example><statement><p>
	Suppose we have polynomial <m>x^2 - 6x + 13</m>.
	Is the <q>number</q> <m>3+2\ci</m> a root?
	To check, substitute
	<m> x = 3+2\ci </m>.
	<md>
		<mrow> \amp \phantom{=} (3+2\ci)^2 - 6(3+2\ci) + 13 </mrow>
		<mrow>
			\amp = (9 + 12\ci + 4(-1)) - 18 - 12\ci + 13
			\amp \amp (\ci^2 = -1)
		</mrow>
		<mrow> \amp = 0. </mrow>
	</md>
	The answer is yes!
	By algebraically combining <m>\ci</m>,
	which is a root of the prototypical <q>unsolvable</q> polynomial equation <m>x^2+1=0</m>,
	with other real numbers,
	we obtain roots of other previously <q>unsolvable</q> polynomial equations.
</p></statement></example>

<p>
It turns out that the result of combining such expressions involving <m>\ci</m> using the four operations of
addition, subtraction, multiplication, and division
can always be simplified using <m>\ci^2 = -1 </m> down to something of the form <m>a + b\ci</m>,
where <m>a,b</m> are real numbers.
</p>

<definition>
	<idx><h>complex</h><h>numbers</h></idx>
	<idx><h>field</h><h>of complex numbers</h></idx>
	<title>The field of complex numbers</title>
	<statement><p>
		The collection <m>\C</m> of all possible algebraic expressions <m>a+b\ci</m>,
		where <m>a,b</m> are real numbers.
		Expressions of this form are called <term>complex numbers</term>.
		In such an expression,
		the number <m>a</m> is called the
		<term>real part</term>
		<idx><h>complex</h><h>numbers</h><h>real part</h></idx>
		<idx><h>real</h><h>part of a complex number</h></idx>
		and the number <m>b</m> is called the
		<term>imaginary part</term><idx><h>complex</h><h>numbers</h><h>imaginary part</h></idx><idx><h>imaginary</h><h>part of a complex number</h></idx>.
	</p></statement>
</definition>

<p><dl>
	<li> <title><m>\Re(z)</m></title> The real part of the complex number <m>z</m>.      </li>
	<li> <title><m>\Im(z)</m></title> The imaginary part of the complex number <m>z</m>. </li>
</dl></p>

<example><title>Real and imaginary parts</title><statement><p><ul>
	<li>
		The complex number <m>-3+\frac{1}{2}\ci</m>
		has real part <m>\Re\left(-3+\frac{1}{2}\ci\right)=-3</m>
		and imaginary part <m>\Im\left(-3+\frac{1}{2}\ci\right)=\frac{1}{2}</m>.
	</li>
	<li>
		The complex number <m>e - \pi\ci = e + (-\pi)\ci</m>
		has real part <m>\Re(e - \pi\ci) = e</m>
		and imaginary part <m>\Im(e - \pi\ci) = -\pi</m>.
	</li>
</ul></p></statement></example>

<remark><title>Real numbers are complex numbers</title>
	<p>
	Every real number <m>a</m> can simultaneously be considered to be a complex number, as
	<me> a = a + 0\ci. </me>
	So the real numbers are precisely those complex numbers that have imaginary part equal to zero.
	(Complex numbers whose <em>real</em> part is equal to zero are called
	<term>purely imaginary</term><idx><h>imaginary</h><h>number</h><h>purely</h></idx>.
	For example, <m>3\ci</m> is purely imaginary.)
	</p>
</remark>

<p>
Roughly speaking, a
<term>field</term><idx><h>field</h><h>of abstract numbers</h></idx>
is a mathematical system of <q>numbers</q> that carries some versions of the four operations
<em>addition</em>, <em>subtraction</em>, <em>multiplication</em>, and <em>division</em>,
and in which these four operations behave arithmetically and algebraically the way we would expect them to behave.
We explore these four operations for the complex numbers,
along with an important new fifth operation,
in the following subsections.
</p>

</subsection>

<subsection xml:id="subsection-complex-appendix-field-ops">
<title>Basic operations with complex numbers</title>

<p>
Here are examples of
adding, subtracting, multiplying, and exponentiating complex numbers.
(We will deal with division afterward.)
Notice it mostly involves just familiar algebra: collecting like terms and FOIL.
</p>

<example><title>Algebraic operations involving complex numbers</title>
	<statement><p><ul>
		<li> <em>Addition:</em> <m> (3+\ci) + (5-3\ci) = 8 - 2\ci </m>. </li>
		<li> <em>Subtraction:</em> <m> (3+\ci) - (5-3\ci) = -2 + 4\ci </m>. </li>
		<li> <em>Multiplication:</em> <m> (3+\ci)(5-3\ci) = 15 - 4\ci - 3(-1) = 18 - 4\ci </m>. </li>
		<li> <em>Power:</em> <m>(3+\ci)^2 = 9 + 6\ci + (-1) = 8 + 6\ci </m>. </li>
		<li> <em>A special multiplication example:</em> <me> (5-3\ci)(5+3\ci) = 25 + 0\ci - 9(-1) = 34. </me> </li>
	</ul></p></statement>
</example>

<p>
The last in the list of examples above is particularly important.
You may recognize it as related to the factorization of a difference of squares.
Since <m>\ci^2 = -1</m>,
multiplying a complex number against its
<q>difference-of-squares-factorization partner</q>
like this always results in a real number.
Because of this,
we'll give this partner a name.
</p>

<definition><title>Complex conjugate</title>
	<idx><h>complex</h><h>conjugate</h></idx>
	<statement><p>
		For complex number <m>z = a + b\ci</m>,
		we define the <term>complex conjugate</term> of <m>z</m> to be
		<me> \cconj{z} = \lcconj{a+b\ci} = a - b\ci. </me>
	</p></statement>
</definition>

<remark><p>
	You should think of complex conjugate as <q>flipping the sign</q> on the imaginary part of the complex number.
	In particular,
	if <m>z = a - b\ci</m> then
	<m>\cconj{z} = \lcconj{a - b\ci} = a + b\ci</m>.
</p></remark>

<example><title>Computing complex conjugates</title><statement><p><ul>
	<li> <m> \lcconj{5+4\ci} = 5 - 4\ci </m>. </li>
	<li> <m> \lcconj{e-\pi\ci} = e + \pi\ci </m>. </li>
</ul></p></statement></example>

</subsection>

<subsection xml:id="subsection-complex-appendix-field-div">
<title>Division of complex nubers</title>

<p> We can use complex conjugates to help us divide complex numbers. </p>

<example><title>Division of complex numbers</title><statement><p>
	To simplify a ratio of complex numbers,
	we can use the conjugate to
	<em>rationalize the denominator</em>,
	as if <m>\ci</m> really were equal to <m>\sqrt{-1}</m>.
	<md>
		<mrow>
			\frac{3+4\ci}{2-3\ci}
			\amp =
			\frac{3+4\ci}{2-3\ci} \cdot \frac{2+3\ci}{2+3\ci}
		</mrow><mrow>
			\amp =
			\frac{(3+4\ci)(2+3\ci)}{(2-3\ci)(2+3\ci)}
		</mrow><mrow>
			\amp =
			\frac{6 + 17 \ci - 12}{2^2 + 3^2}
		</mrow><mrow>
			\amp =
			\frac{-6 + 17 \ci}{13}
		</mrow><mrow>
			\amp =
			-\frac{6}{13} + \frac{17}{13}\, \ci.
		</mrow>
	</md>
</p></statement></example>

<paragraphs><title>Pattern</title><p>
	In general, division of complex numbers follows the pattern
	<me>
		\frac{a+b\ci}{c+d\ci}
		= \frac{a+b\ci}{c+d\ci} \cdot \frac{c-d\ci}{c-d\ci}
		= \left(\frac{ac+bd}{c^2+d^2}\right) + \left(\frac{bc-ad}{c^2+d^2}\right) \; \ci.
	</me>
</p></paragraphs>

<p> Since we can divide, we can also reciprocate. </p>

<example xml:id="example-complex-field-reciprocal"><title>Reciprocal of a complex number</title><statement><p>
	Let's compute the reciprocal of <m>3+2\ci</m>.
	<me> \inv{(3+2\ci)} = \frac{1}{3+2\ci} = \frac{1+0\ci}{3+2\ci} \cdot \frac{3-2\ci}{3-2\ci} = \frac{3}{13} - \frac{2}{13}\, \ci. </me>
	If we multiply a number and its reciprocal,
	we would expect to get <m>1</m> as the result.
	<md>
		<mrow>
			(3+2\ci)\inv{(3+2\ci)}
			\amp
			= (3+2\ci)\left(\frac{3}{13} - \frac{2}{13}\, \ci\right)
		</mrow><mrow>
			\amp
			= \frac{9}{13} - \frac{6}{13}\, \ci + \frac{6}{13}\, \ci - \frac{4}{13} \cdot (-1)
		</mrow><mrow>
			\amp
			= 1 + 0 \ci
		</mrow><mrow>
			\amp
			= 1.
		</mrow>
	</md>
	It worked!
</p></statement></example>

<p>
There is a pattern to this reciprocal example,
but it will have to wait until after
<xref ref="proposition-appendix-complex-field-modulus-properties" />.
</p>

</subsection>

<subsection xml:id="subsection-complex-appendix-field-props">
<title> Properties of complex numbers </title>

<p>
Since the operations of
addition, subtraction, multiplication, and division
of complex numbers are built on following our usual algebra rules on expressions involving the <q>variable</q> <m>\ci</m>
(along with the extra rule <m>\ci^2 = -1</m>),
there is no need to restate all those usual algebra rules.
So we will focus on the new operation of complex conjugation.
</p>

<proposition xml:id="proposition-appendix-complex-field-conjugate-properties">
	<title>Properties of complex conjugates</title>
	<statement><p>
		The following are valid rules of algebra involving the complex conjugation operation.
		Let <m>w</m> and <m>z</m> represent arbitrary complex numbers,
		and let <m>k</m> represent an arbitrary real number.
		<ol>
			<li>
				Conjugating a real number has no effect.
				That is, <m>\cconj{k} = k</m>.
			</li>
			<li>
				The conjuate of a sum is the sum of the conjugates.
				That is, <m>\lcconj{w+z} = \cconj{w} + \cconj{z}. </m>
			</li>
			<li xml:id="proposition-appendix-complex-field-conjugate-properties-product">
				The conjugate of a product is the product of the conjugates.
				That is, <m>\lcconj{wz} = \cconj{w}\cconj{z}. </m>
			</li>
			<li>
				The conjugate of a <q>scalar multiple</q> is the <q>scalar multiple</q> of the conjugate.
				That is, <m>\lcconj{kz} = k\cconj{z}. </m>
			</li>
			<li>
				The conjugate of a quotient is the quotient of the conjugates.
				That is, <m>\lcconj{w/z} = \cconj{w} / \cconj{z}</m>.
			</li>
			<li>
				The conjugate of a reciprocal is the reciprocal of the conjugate.
				That is, <m>\lcconj{1/z} = 1 / \cconj{z}</m>.
			</li>
			<li>
				For every nonzero, integer exponent,
				the conjugate of that power is the power of the conjugate.
				That is, <m>\lcconj{z^n} = \cconj{z}^n</m>.
			</li>
		</ol>
	</p></statement>
</proposition>

<p> Considering how a complex number interacts with its own conjugate yields several important patterns. </p>

<proposition xml:id="proposition-appendix-complex-field-conjugate-relative-properties">
	<title>Relative properties of complex conjugates</title>
	<statement>
		<p>
		A complex number <m>z</m> satisfies the following special relationships with its own conjugate.
		<ol>
			<li>
				The conjugate of a conjugate is the original complex number.
				That is, <m>\lcconj{\cconj{z}} = z</m>.
			</li>
			<li xml:id="proposition-appendix-complex-field-conjugate-relative-properties-real-iff">
				A complex number is actually real
				(<ie /> has imaginary part <m>0</m>)
				if and only if it is equal to its own conjugate.
				That is, <m>z</m> is real if and only if <m>\cconj{z} = z</m>.
			</li>
			<li>
				A complex number is purely imaginary
				(<ie /> has real part <m>0</m>)
				if and only if it is equal to the negative of its own conjugate.
				That is, <m>z</m> is purely imaginary if and only if <m>\cconj{z} = -z</m>.
			</li>
			<li>
				Combining a complex number with its conjugate using addition or subtraction returns twice the real part or twice the imaginary part times <m>\ci</m>,
				respectively.
				That is,
				<md><mrow>
					z + \cconj{z} \amp = 2\cdot\Re(z), \amp
					z - \cconj{z} = 2\cdot\Im(z)\cdot\ci.
				</mrow></md>
			</li>
			<li xml:id="proposition-appendix-complex-field-conjugate-relative-properties-times">
				Multiplying a complex number and its complex conjugate always results in a real number,
				equal to the sum of the squares of the real and imaginary parts.
				That is, if <m>z = a + b\ci</m>,
				then <m>z\cconj{z} = a^2 + b^2</m>.
			</li>
		</ol>
		</p>
	</statement>
</proposition>

<p>
The sum-of-squares pattern in
<xref ref="proposition-appendix-complex-field-conjugate-relative-properties-times">Statement</xref>
of
<xref ref="proposition-appendix-complex-field-conjugate-relative-properties" />
has a connection to geometry via Pythagoras that we will explore in
<xref ref="section-complex-appendix-plane" />.
(And by the time you are reading this appendix,
you may already have encountered the sum-of-squares formula's connection to geometry in a linear algebra context in
<xref ref="chapter-vector-geom" />.)
For now, we will give a version of this formula a name.
</p>

<definition>
	<title>Complex modulus</title>
	<idx><h>complex</h><h>modulus</h></idx>
	<statement><p>
		For complex number <m>z = a + b\ci</m>,
		the real number
		<m>\cmodulus{z} = \sqrt{a^2 + b^2}</m>
		is called the
		<term>modulus</term>
		<idx><h>complex</h><h>modulus</h></idx>
		<idx><h>modulus (of a complex number)</h></idx>
		of <m>z</m>.
	</p></statement>
</definition>

<proposition xml:id="proposition-appendix-complex-field-modulus-properties">
	<title>Properties of the complex modulus</title>
	<statement><p>
		The following are valid rules of algebra involving the complex modulus.
		Let <m>w</m> and <m>z</m> represent arbitrary complex numbers,
		and let <m>k</m> represent an arbitrary real number.
		<ol>
			<li xml:id="proposition-appendix-complex-field-modulus-properties-modulus-squared">
				The square of the modulus is equal to the product of the complex number with its own conjugate.
				That is, <m>\cmodulus{z}^2 = z\cconj{z}</m>.
			</li>
			<li xml:id="proposition-appendix-complex-field-modulus-properties-nonneg">
				A modulus is never negative,
				and only zero has modulus zero.
				That is, <m>\cmodulus{z} \ge 0</m>,
				with <m>\cmodulus{z} = 0</m> if and only if <m>z=0</m>.
			</li>
			<li>
				A complex number and its conjugate have the same modulus.
				That is, <m>\cmodulus{\cconj{z}} = \cmodulus{z}</m>.
			</li>
			<li> The modulus of a real number is equal to the absolute value of that number. </li>
			<li>
				The modulus of a product is the product of the moduli.
				That is, <m>\cmodulus{wz} = \cmodulus{w}\cmodulus{z}</m>.
			</li>
			<li>
				The modulus of a <q>scalar multiple</q> is the absolute <q>scalar multiple</q> of the modulus.
				That is, <m>\cmodulus{kz} = \abs{k}\cmodulus{z}</m>,
				where <m>\abs{k}</m> is the regular absolute value of the real number <m>k</m>.
			</li>
			<li>
				The modulus of a quotient is the quotient of the moduli.
				That is, <m>\cmodulus{w/z} = \cmodulus{w}/\cmodulus{z}</m>.
			</li>
			<li>
				The modulus of a reciprocal is the reciprocal of the modulus.
				That is, <m>\cmodulus{1/z} = 1/\cmodulus{z}</m>.
			</li>
			<li xml:id="proposition-appendix-complex-field-modulus-properties-power">
				For every nonzero, integer exponent,
				the modulus of that power is the power of the modulus.
				That is, <m>\cmodulus{z^n} = \cmodulus{z}^n</m>.
			</li>
			<li>
				The modulus satisfies the <term>Triangle Inequality</term>:
				<m>\cmodulus{w + z} \le \cmodulus{w} + \cmodulus{z}</m>.
			</li>
		</ol>
	</p></statement>
</proposition>

<paragraphs><title>Pattern</title><p>
	We can use
	<xref ref="proposition-appendix-complex-field-modulus-properties-modulus-squared">Statement</xref>
	of
	<xref ref="proposition-appendix-complex-field-modulus-properties" />
	to help us reciprocate:
	<md><mrow>
		\cmodulus{z}^2 \amp = z\cconj{z}
		\amp \amp \implies \amp
		\inv{z} \amp = \frac{\cconj{z}}{\cmodulus{z}^2}.
	</mrow></md>
</p></paragraphs>

<example><title>Reciprocal of a complex number, revisited</title><statement>
	<p>
	Let's recompute the reciprocal of <m>3+2\ci</m>
	(from <xref ref="example-complex-field-reciprocal" />).
	</p>
	<p>
	We have
	<me> \cmodulus{3+2\ci}^2 = 3^2 + 2^2 = 13, </me>
	and so
	<me> \inv{(3+2\ci)} = \frac{\lcconj{3+2\ci}}{\cmodulus{3+2\ci}^2} = \frac{3-2\ci}{13} = \frac{3}{13} - \frac{2}{13}\, \ci, </me>
	which is the same reciprocal as previously calculated in
	<xref ref="example-complex-field-reciprocal" />.
	</p>
</statement></example>

</subsection>

<subsection xml:id="subsection-complex-appendix-field-poly">
<title> Complex polynomials </title>

<introduction><p>
	The most important property of the field of complex numbers is that by merely inventing a solution to <em>one</em> previously unsolvable polynomial equation
	(<ie /> the imaginary solution <m>\ci</m> to <m>x^2 + 1 = 0</m>),
	we have actually created solutions to <em>all</em> polynomial equations.
</p></introduction>

<p>
Now that we know how to perform arithmetic with complex numbers,
we can expand to doing some algebra.
A
<term>complex polynomial</term>
<idx><h>complex</h><h>polynomial</h></idx>
is just a polynomial where we allow the coefficients to be complex numbers,
and assume the variable to represent an unknown complex number.
</p>

<example><title>Checking a solution to a complex polynomial</title><statement><p>
	Is <m>z = 4-\ci</m> a solution to the complex polynomial equation <m>z^2 + \ci z + (-16+4\ci)=0</m>?
	<md>
		<mrow> \amp \phantom{=} (4-\ci)^2 + \ci (4-\ci) + (-16+4\ci) </mrow>
		<mrow> \amp = \bigl[16 - 8\ci + (-1)\bigr] + \bigl[4\ci - (-1)\bigr] + (-16+4\ci) </mrow>
		<mrow> \amp = 0. </mrow>
	</md>
	Yes, <m>z = 4-\ci</m> is a solution to <m>z^2 + \ci z + (-16+4\ci)</m>.
</p></statement></example>

<theorem xml:id="theorem-complex-fund-thm-alg-complex">
	<idx><h>Fundamental Theorem of Algebra</h><h>complex version</h></idx>
	<title>The Fundamental Theorem of Algebra (Complex Version)</title>
	<statement><p>
		If <m>p(z)</m> is a complex polynomial of degree <m>n \ge 1</m>,
		then the polynomial equation <m>p(z) = 0</m> has <em>exactly</em> <m>n</m> roots
		(where repeated roots are counted multiple times,
		according to the number of times that root is repeated).
	</p></statement>
</theorem>

<p>
Because determining roots of a polynomial is equivalent to factoring that polynomial,
we can reinterpret this theorem in terms of factoring.
</p>

<corollary xml:id="corollary-complex-fund-thm-alg-complex-factoring"><statement><p>
	Every complex polynomial <m>p(z)</m> can be <em>completely factored</em> as
	<me> p(z) = w_0 (z-w_1)(z-w_2) \dotsm (z-w_n), </me>
	for some constant complex numbers
	<m>w_0,w_1,w_2,\dotsc,w_n</m>,
	where <m>n</m> is the degree of <m>p(z)</m>.
</p></statement></corollary>

<p>
We can also use this complex version of the Fundamental Theorem to refine the real version
(<xref ref="theorem-complex-fund-thm-alg-reals"/>),
since a real polynomial can be considered to be a complex polynomial that just happens to have purely real numbers as coefficients.
</p>

<corollary><statement><p>
	If <m>p(x)</m> is a real polynomial of degree <m>n \ge 1</m>,
	then the polynomial equation <m>p(x) = 0</m> has <em>exactly</em> <m>n</m> roots when we allow complex numbers as roots
	(and where again, repeated roots are counted multiple times).
</p></statement></corollary>

<example xml:id="example-complex-field-cubic-fully-factored">
	<title>Roots of a cubic polynomial</title>
	<statement><p>
		Consider the cubic polynomial equation
		<md>
			<mrow xml:id="equation-complex-field-cubic-fully-factored" tag="star">
				x^3 + 3x^2 + 2x - 6 = 0.
			</mrow>
		</md>
		We can guess one root:
		<m>x=1</m> solves this equation.
		This means that <m>x-1</m> is a factor of this polynomial.
		Using long division of polynomials,
		we could calculate
		<me> \frac{x^3 + 3x^2 + 2x - 6}{x-1} = x^2+4x+6, </me>
		so that
		<me> x^3 + 3x^2 + 2x - 6 = (x-1)(x^2+4x+6). </me>
		So to determine the other roots of
		<xref ref="equation-complex-field-cubic-fully-factored" />,
		we only need to determine the roots of
		<m>x^2+4x+6 = 0</m>.
		As a <em>real</em> polynomial,
		this quadratic factor is irreducible
		(<ie /> has no roots).
		However, as a <em>complex</em> polynomial,
		we can use the quadratic formula:
		<md>
			<mrow> x \amp = \frac{-4 \pm \sqrt{16 - 4 \cdot 1 \cdot 6}}{2} </mrow>
			<mrow> \amp = \frac{-4 \pm \sqrt{-8}}{2} </mrow>
			<mrow> \amp = \frac{-4 \pm \sqrt{-1}\sqrt{2}\sqrt{4}}{2} </mrow>
			<mrow> \amp = -2 \pm \ci\sqrt{2}. </mrow>
		</md>
		Therefore, the degree-three polynomial equation in
		<xref ref="equation-complex-field-cubic-fully-factored" />
		does indeed have precisely three roots:
		<me> x = -1, -2+\ci\sqrt{2}, -2-\ci\sqrt{2}. </me>
		And the cubic polynomial in
		<xref ref="equation-complex-field-cubic-fully-factored" />
		can be fully factored as
		<me> x^3 + 3x^2 + 2x - 6 = (x-1)\bbrac{x - (-2+\ci\sqrt{2})}\bbrac{x - (-2-\ci\sqrt{2})}. </me>
	</p></statement>
</example>

</subsection>

</section>
